@prefix : <http://www.semanticweb.org/owl/owlapi/turtle#> .
@prefix owl: <http://www.w3.org/2002/07/owl#> .
@prefix rdf: <http://www.w3.org/1999/02/22-rdf-syntax-ns#> .
@prefix xml: <http://www.w3.org/XML/1998/namespace> .
@prefix xsd: <http://www.w3.org/2001/XMLSchema#> .
@prefix bppo: <http://www.w3id.org/ppon/bppo#> .
@prefix lppo: <http:/w3id.org/ppon/lppo.owl> .
@prefix qudt: <http://qudt.org/schema/qudt#> .
@prefix rdfs: <http://www.w3.org/2000/01/rdf-schema#> .
@prefix skos: <http://www.w3.org/2004/02/skos/core#> .
@base <http://www.semanticweb.org/owl/owlapi/turtle#> .

[ rdf:type owl:Ontology
 ] .

#################################################################
#    Annotation properties
#################################################################

###  http://qudt.org/schema/qudt#unit
qudt:unit rdf:type owl:AnnotationProperty .


###  http://www.w3.org/2004/02/skos/core#definition
skos:definition rdf:type owl:AnnotationProperty .


###  http://www.w3id.org/ppon/bppo#hasGUID
bppo:hasGUID rdf:type owl:AnnotationProperty .


#################################################################
#    Data properties
#################################################################

###  http:/w3id.org/ppon/lppo.owlactivePower
lppo:activePower rdf:type owl:DatatypeProperty ;
                 rdfs:domain lppo:LightingFixtureElectricalProperties ;
                 rdfs:range xsd:decimal ;
                 qudt:unit qudt:W ,
                           qudt:lm ,
                           qudt:percentage ;
                 rdfs:label "Active Power" ;
                 skos:definition """Consumption of the power corresponding to
the dim level of the luminaire. It is presented as a table of
power (W) related to the luminous flux emitted (lm) or the percentage of dimming (%).""" ;
                 bppo:hasGUID "0zjByQSTX24wsxTI25Lzj$" .


###  http:/w3id.org/ppon/lppo.owlapparentLoad
lppo:apparentLoad rdf:type owl:DatatypeProperty ;
                  rdfs:domain lppo:LightingFixtureElectricalProperties ;
                  rdfs:range xsd:decimal ;
                  qudt:unit qudt:VA ;
                  rdfs:label "Apparent Load" ;
                  skos:definition "Apparent load of the product." ;
                  bppo:hasGUID "2FA0ih18LF_uKt46e5ErIv" .


###  http:/w3id.org/ppon/lppo.owlbackupSupplySystem
lppo:backupSupplySystem rdf:type owl:DatatypeProperty ;
                        rdfs:domain lppo:LightingFixtureEmergencyLightingProperties ;
                        rdfs:range xsd:string ;
                        rdfs:label "Backup Supply System" ;
                        skos:definition "Specifies the emergency power backup: battery, generator, etc." ;
                        bppo:hasGUID "2Yq5DQRXP7efr3cQyq8sqS" .


###  http:/w3id.org/ppon/lppo.owlcompensationType
lppo:compensationType rdf:type owl:DatatypeProperty ;
                      rdfs:domain lppo:LightingFixtureElectricalProperties ;
                      rdfs:range xsd:string ;
                      rdfs:label "Compensation type" ;
                      skos:definition """Identifies the form of compensation used for
power factor correction and radio interference suppression.""" ;
                      bppo:hasGUID "3krkQTVbv0$g9Xj9eYC6nh" .


###  http:/w3id.org/ppon/lppo.owlcutOutDiameter
lppo:cutOutDiameter rdf:type owl:DatatypeProperty ;
                    rdfs:domain lppo:LightingFixtureMechanicalProperties ;
                    rdfs:range xsd:decimal ;
                    qudt:unit qudt:MilliM ;
                    rdfs:label "Cut-Out Diameter" ;
                    skos:definition "Diameter of the cut-out hole (for recessed or flush mount)." ;
                    bppo:hasGUID "2A6xVlUTj9QP1G$qb4FiWv" .


###  http:/w3id.org/ppon/lppo.owlcuttingOutLength
lppo:cuttingOutLength rdf:type owl:DatatypeProperty ;
                      rdfs:domain lppo:LightingFixtureMechanicalProperties ;
                      rdfs:range xsd:decimal ;
                      qudt:unit qudt:MilliM ;
                      rdfs:label "Cutting Out Length" ;
                      skos:definition "Length of the cut-out hole (for recessed or flush mount)." ;
                      bppo:hasGUID "2VEYAfd7j4FQtJgAb_riA5" .


###  http:/w3id.org/ppon/lppo.owlcuttingOutWidth
lppo:cuttingOutWidth rdf:type owl:DatatypeProperty ;
                     rdfs:domain lppo:LightingFixtureMechanicalProperties ;
                     rdfs:range xsd:decimal ;
                     qudt:unit qudt:MilliM ;
                     rdfs:label "Cutting Out Width" ;
                     skos:definition "Width of the cut-out hole (for recessed or flush mount)." ;
                     bppo:hasGUID "2pFfNBOuv1Tf_RTQpYktGL" .


###  http:/w3id.org/ppon/lppo.owldistributionType
lppo:distributionType rdf:type owl:DatatypeProperty ;
                      rdfs:domain lppo:LightingFixturePhotometricProperties ;
                      rdfs:range xsd:string ;
                      rdfs:label "Type of Distribution" ;
                      skos:definition "Classification based on upper/lower light flux." ;
                      bppo:hasGUID "28T0Q968jDwv yxAshmZRwz" .


###  http:/w3id.org/ppon/lppo.owldownwardFluxFraction
lppo:downwardFluxFraction rdf:type owl:DatatypeProperty ;
                          rdfs:domain lppo:LightingFixturePhotometricProperties ;
                          rdfs:range xsd:decimal ;
                          qudt:unit qudt:PERCENT ;
                          rdfs:label "Downward Flux Fraction" ;
                          skos:definition "Ratio of downward flux to total luminaire flux." ;
                          bppo:hasGUID "3O71lbRGPDpOk4BrfOhVAO" .


###  http:/w3id.org/ppon/lppo.owlemergencyLightingType
lppo:emergencyLightingType rdf:type owl:DatatypeProperty ;
                           rdfs:domain lppo:LightingFixtureEmergencyLightingProperties ;
                           rdfs:range xsd:string ;
                           rdfs:label "Dedicated Emergency Lighting Type" ;
                           skos:definition "Type of emergency luminaire: exit, guide, evacuation, reference light, etc." ;
                           bppo:hasGUID "3Q6UsxAKD0Q8mO0x0ZsmhD" .


###  http:/w3id.org/ppon/lppo.owlemergencyTestMethod
lppo:emergencyTestMethod rdf:type owl:DatatypeProperty ;
                         rdfs:domain lppo:LightingFixtureEmergencyLightingProperties ;
                         rdfs:range xsd:string ;
                         rdfs:label "Emergency Testing Method" ;
                         skos:definition "Describes the method used to test emergency functionality: manual, self-test, etc." ;
                         bppo:hasGUID "2qgqLlM2b91wjREM3dUep2" .


###  http:/w3id.org/ppon/lppo.owlemergencyUnitIntegrated
lppo:emergencyUnitIntegrated rdf:type owl:DatatypeProperty ;
                             rdfs:domain lppo:LightingFixtureEmergencyLightingProperties ;
                             rdfs:range xsd:boolean ;
                             rdfs:label "Emergency Unit Integrated" ;
                             skos:definition "Specifies whether emergency functionality is integrated in the luminaire." ;
                             bppo:hasGUID "3pJBuEixPAV9f0wTnl2cOM" .


###  http:/w3id.org/ppon/lppo.owlheight
lppo:height rdf:type owl:DatatypeProperty ;
            rdfs:domain lppo:LightingFixtureMechanicalProperties ;
            rdfs:range xsd:decimal ;
            qudt:unit qudt:MilliM ;
            rdfs:label "Height" ;
            skos:definition """Height of the housing of the luminaire or sensing 
    device. Corresponds to z-axis, gamma angle 180° and
180° vertical of the light distribution curve. This
definition is regardless of orientation of luminaires.
See Figure 1.""" ;
            bppo:hasGUID "19Z9XKYDT4p8HR0ZbD$wO_" .


###  http:/w3id.org/ppon/lppo.owllength
lppo:length rdf:type owl:DatatypeProperty ;
            rdfs:domain lppo:LightingFixtureMechanicalProperties ;
            rdfs:range xsd:decimal ;
            qudt:unit qudt:MilliM ;
            rdfs:label "Length" ;
            skos:definition """Length of the housing of the luminaire or sensing device.
Length is set parallel to the C90-C270 plane.
Corresponds to y-axis and with 90° horizontal of the
Light Distribution Curve. This definition is regardless
of orientation of luminaires. See Figure 1.""" ;
            bppo:hasGUID "1uJglYpRnFpQ4tStHaR2Pf" .


###  http:/w3id.org/ppon/lppo.owllightOutputRatio
lppo:lightOutputRatio rdf:type owl:DatatypeProperty ;
                      rdfs:domain lppo:LightingFixturePhotometricProperties ;
                      rdfs:range xsd:decimal ;
                      qudt:unit qudt:PERCENT ;
                      rdfs:label "Light Output Ratio" ;
                      skos:definition "Ratio of luminaire luminous flux to the sum of individual light sources fluxes." ;
                      bppo:hasGUID "2gMYX1hkHEE8kQmgimay3h" .


###  http:/w3id.org/ppon/lppo.owlluminousEfficacy
lppo:luminousEfficacy rdf:type owl:DatatypeProperty ;
                      rdfs:domain lppo:LightingFixturePhotometricProperties ;
                      rdfs:range xsd:decimal ;
                      qudt:unit qudt:LumenPerWatt ;
                      rdfs:label "Luminous Efficacy" ;
                      skos:definition "Ratio of luminous flux emitted to power absorbed." ;
                      bppo:hasGUID "1QmFILGbX6_BfU63rG5mrh" .


###  http:/w3id.org/ppon/lppo.owloverallDiameter
lppo:overallDiameter rdf:type owl:DatatypeProperty ;
                     rdfs:domain lppo:LightingFixtureMechanicalProperties ;
                     rdfs:range xsd:decimal ;
                     qudt:unit qudt:MilliM ;
                     rdfs:label "Overall Diameter" ;
                     skos:definition "Overall diameter of the housing of the luminaire or sensing device." ;
                     bppo:hasGUID "2GZ1YB8enFVhDHOKgLc$BU" .


###  http:/w3id.org/ppon/lppo.owlpowerFactor
lppo:powerFactor rdf:type owl:DatatypeProperty ;
                 rdfs:domain lppo:LightingFixtureElectricalProperties ;
                 rdfs:range xsd:decimal ;
                 rdfs:label "Power Factor" ;
                 skos:definition """Ratio of the amount of the active power to the
apparent power at 100 % load. See also IEC 80000-6.""" ;
                 bppo:hasGUID "3LBrQkLDDFheBOxrGk8Zr_" .


###  http:/w3id.org/ppon/lppo.owlratedInputPower
lppo:ratedInputPower rdf:type owl:DatatypeProperty ;
                     rdfs:domain lppo:LightingFixtureElectricalProperties ;
                     rdfs:range xsd:decimal ;
                     qudt:unit qudt:W ;
                     rdfs:label "Rated Input Power" ;
                     skos:definition """Input power consumed by the light source(s),
control gear and control circuit in or associated
with a luminaire including any standby
power when the luminaire is turned on.""" ;
                     bppo:hasGUID "17a067965CqhDelQ$Y3mcP" .


###  http:/w3id.org/ppon/lppo.owlrecessedRequiredDepth
lppo:recessedRequiredDepth rdf:type owl:DatatypeProperty ;
                           rdfs:domain lppo:LightingFixtureMechanicalProperties ;
                           rdfs:range xsd:decimal ;
                           qudt:unit qudt:MilliM ;
                           rdfs:label "Recessed Required Depth" ;
                           skos:definition """Required minimum installation depth, height of the
invisible / hidden mounting part of the luminaire (for
recessed or flush mount).""" ;
                           bppo:hasGUID "1RIsLltoX1whNaYkaCoHXJ" .


###  http:/w3id.org/ppon/lppo.owlsensingAngle
lppo:sensingAngle rdf:type owl:DatatypeProperty ;
                  rdfs:domain lppo:LightingFixtureSensingDeviceProperties ;
                  rdfs:range xsd:decimal ;
                  qudt:unit qudt:DegreeAngle ;
                  rdfs:label "Angle of Detection" ;
                  skos:definition "Angular span over which motion or light is detected." ;
                  bppo:hasGUID "3bSKg4LUz5N8OoMR0cLgfS" .


###  http:/w3id.org/ppon/lppo.owlsensingField
lppo:sensingField rdf:type owl:DatatypeProperty ;
                  rdfs:domain lppo:LightingFixtureSensingDeviceProperties ;
                  rdfs:range xsd:string ;
                  rdfs:label "Field of Detection" ;
                  skos:definition "Shape or type of detection field (e.g., circular, rectangular)." ;
                  bppo:hasGUID "0WyJSYrS99cQ8InU7X3j2V" .


###  http:/w3id.org/ppon/lppo.owlsensingFunction
lppo:sensingFunction rdf:type owl:DatatypeProperty ;
                     rdfs:domain lppo:LightingFixtureSensingDeviceProperties ;
                     rdfs:range xsd:string ;
                     rdfs:label "Sensing Function" ;
                     skos:definition "Specifies the type of sensor function integrated (e.g., presence detection, daylight harvesting)." ;
                     bppo:hasGUID "2Zds3bmON4TfKejdVo2nG7" .


###  http:/w3id.org/ppon/lppo.owlsensingRange
lppo:sensingRange rdf:type owl:DatatypeProperty ;
                  rdfs:domain lppo:LightingFixtureSensingDeviceProperties ;
                  rdfs:range xsd:decimal ;
                  qudt:unit qudt:Meter ;
                  rdfs:label "Range of Detection" ;
                  skos:definition "Maximum detection distance of the integrated sensor." ;
                  bppo:hasGUID "1TwTzRQ3z3U8J8R2HKaaRA" .


###  http:/w3id.org/ppon/lppo.owlsensingTechnology
lppo:sensingTechnology rdf:type owl:DatatypeProperty ;
                       rdfs:domain lppo:LightingFixtureSensingDeviceProperties ;
                       rdfs:range xsd:string ;
                       rdfs:label "Sensing Technology" ;
                       skos:definition "Technology used in the sensing system (e.g., passive infrared, microwave)." ;
                       bppo:hasGUID "3nVokP4n11nPdVycecrkFZ" .


###  http:/w3id.org/ppon/lppo.owlstandbyPower
lppo:standbyPower rdf:type owl:DatatypeProperty ;
                  rdfs:domain lppo:LightingFixtureElectricalProperties ;
                  rdfs:range xsd:decimal ;
                  qudt:unit qudt:W ;
                  rdfs:label "Standby Power" ;
                  skos:definition "Power consumed when luminaire is switched off, including parasitic consumption." ;
                  bppo:hasGUID "0TzE4sMDv1pwfygK1xxjm5" .


###  http:/w3id.org/ppon/lppo.owlsuitableForEmergencyLighting
lppo:suitableForEmergencyLighting rdf:type owl:DatatypeProperty ;
                                  rdfs:domain lppo:LightingFixtureEmergencyLightingProperties ;
                                  rdfs:range xsd:boolean ;
                                  rdfs:label "Suitable for Emergency Lighting" ;
                                  skos:definition "Indicates whether the luminaire can be used in emergency lighting applications." ;
                                  bppo:hasGUID "0nXXpyMbD4QgzHiMoFE$Kf" .


###  http:/w3id.org/ppon/lppo.owlweight
lppo:weight rdf:type owl:DatatypeProperty ;
            rdfs:domain lppo:LightingFixtureMechanicalProperties ;
            rdfs:range xsd:decimal ;
            qudt:unit qudt:KiloGM ;
            rdfs:label "Weight" ;
            skos:definition "Weight of the luminaire or sensing device." ;
            bppo:hasGUID "1RPyGAgMf4hRTZ0DogLFnU" .


###  http:/w3id.org/ppon/lppo.owlwidth
lppo:width rdf:type owl:DatatypeProperty ;
           rdfs:domain lppo:LightingFixtureMechanicalProperties ;
           rdfs:range xsd:decimal ;
           qudt:unit qudt:MilliM ;
           rdfs:label "Width" ;
           skos:definition """Width of the housing of the luminaire or sensingdevice.
Width is set parallel to the C0-C180 plane.
Corresponds to the x-axis and with 0° horizontal of
the Light Distribution Curve. This definition is
regardless of orientation of luminaires. See Figure 1.""" ;
           bppo:hasGUID "1dPvrZN3vEIB0n0vwYvDcX" .


#################################################################
#    Classes
#################################################################

###  http:/w3id.org/ppon/lppo.owlLightingFixtureElectricalProperties
lppo:LightingFixtureElectricalProperties rdf:type owl:Class ;
                                         rdfs:subClassOf lppo:LightingFixtureProperties .


###  http:/w3id.org/ppon/lppo.owlLightingFixtureEmergencyLightingProperties
lppo:LightingFixtureEmergencyLightingProperties rdf:type owl:Class ;
                                                rdfs:subClassOf lppo:LightingFixtureProperties .


###  http:/w3id.org/ppon/lppo.owlLightingFixtureMechanicalProperties
lppo:LightingFixtureMechanicalProperties rdf:type owl:Class ;
                                         rdfs:subClassOf lppo:LightingFixtureProperties .


###  http:/w3id.org/ppon/lppo.owlLightingFixturePhotometricProperties
lppo:LightingFixturePhotometricProperties rdf:type owl:Class ;
                                          rdfs:subClassOf lppo:LightingFixtureProperties .


###  http:/w3id.org/ppon/lppo.owlLightingFixtureProperties
lppo:LightingFixtureProperties rdf:type owl:Class ;
                               rdfs:comment "A class representing a lighting fixture, including mechanical, electrical, photometric, emergency, sensing, mounting, marketing, and maintenance properties." ;
                               rdfs:label "Lighting Fixture Properties" .


###  http:/w3id.org/ppon/lppo.owlLightingFixtureSensingDeviceProperties
lppo:LightingFixtureSensingDeviceProperties rdf:type owl:Class ;
                                            rdfs:subClassOf lppo:LightingFixtureProperties .


###  Generated by the OWL API (version 4.5.29.2024-05-13T12:11:03Z) https://github.com/owlcs/owlapi
