@prefix : <http://www.w3id.org/ppon/bppo#> .
@prefix dc: <http://purl.org/dc/elements/1.1/> .
@prefix bpo: <http://www.w3id.org/bpo#> .
@prefix owl: <http://www.w3.org/2002/07/owl#> .
@prefix rdf: <http://www.w3.org/1999/02/22-rdf-syntax-ns#> .
@prefix xml: <http://www.w3.org/XML/1998/namespace> .
@prefix xsd: <http://www.w3.org/2001/XMLSchema#> .
@prefix rdfs: <http://www.w3.org/2000/01/rdf-schema#> .
@prefix skos: <http://www.w3.org/2004/02/skos/core#> .
@base <http://www.w3id.org/ppon/bppo> .

<http://www.w3id.org/ppon/bppo> rdf:type owl:Ontology ;
                                 owl:versionIRI <http://www.w3id.org/ppon/bppo/1.0> ;
                                 rdfs:comment """The Building Product Property Ontology (BPPO) provides a vocabulary to define the properties for the products used in the construction industry. The ontology has been developed in accordance with the standard ISO23386:2020. 

The namespace for BPPO terms is http://www.w3id.org/ppon/bppo#

The suggested prefix for the BPPO namespace is bppo."""@en .

#################################################################
#    Object Properties
#################################################################

###  http://www.w3.org/2004/02/skos/core#related
skos:related rdf:type owl:ObjectProperty .


###  http://www.w3id.org/ppon/bppo#compatibleWith
:compatibleWith rdf:type owl:ObjectProperty ;
                rdfs:domain :Property ;
                rdfs:range :InterconnectedDictionary ;
                rdfs:comment "This property is used for compatibility between already existing properties." ;
                rdfs:label "relation of the property in the interconnected dictionaries" .


###  http://www.w3id.org/ppon/bppo#countryOfUse
:countryOfUse rdf:type owl:ObjectProperty ;
              rdfs:domain :Property ;
              rdfs:comment "Country in which the property is used." ;
              rdfs:label "Country of use" .


###  http://www.w3id.org/ppon/bppo#language
:language rdf:type owl:ObjectProperty ;
          rdfs:domain :Property ;
          rdfs:range dc:Language .


###  http://www.w3id.org/ppon/bppo#memberOf
:memberOf rdf:type owl:ObjectProperty ;
          rdfs:domain :Property ;
          rdfs:range :PropertyGroup ;
          rdfs:comment "This property describes the product property is a member of property group." ;
          rdfs:label "member of" .


###  http://www.w3id.org/ppon/bppo#propertyOf
:propertyOf rdf:type owl:ObjectProperty ;
            rdfs:domain :Property ;
            rdfs:range bpo:Product ;
            rdfs:comment "This property describes a property is used to decribe the characteristics of product." ;
            rdfs:label "property of" .


###  http://www.w3id.org/ppon/bppo#propertyStatus
:propertyStatus rdf:type owl:ObjectProperty ;
                rdfs:domain :Property ;
                rdfs:range :Status ;
                rdfs:comment "The property describes the status of the property during its life cycle." ;
                rdfs:label "Status" .


###  http://www.w3id.org/ppon/bppo#replacedBy
:replacedBy rdf:type owl:ObjectProperty ;
            rdfs:domain :Property ;
            rdfs:range :Property ;
            rdfs:comment "Identifier of the replacing property (or properties)." ;
            rdfs:label "Replaced by" .


#################################################################
#    Data properties
#################################################################

###  http://www.w3id.org/ppon/bppo#dataType
:dataType rdf:type owl:DatatypeProperty ;
          rdfs:domain :Property ;
          rdfs:comment "Format for expressing the value of the property. This can be understood as the storage type from a software perspective. In case of a dynamic property the value of this attribute is the datatype of the result of the calculation by the formula" ;
          rdfs:label "Data Type" .


###  http://www.w3id.org/ppon/bppo#dateOfActivation
:dateOfActivation rdf:type owl:DatatypeProperty ;
                  rdfs:domain :Property ;
                  rdfs:range xsd:dateTime ;
                  rdfs:comment "Date after when the property can be used." ;
                  rdfs:label "Date of activation" .


###  http://www.w3id.org/ppon/bppo#dateOfCreation
:dateOfCreation rdf:type owl:DatatypeProperty ;
                rdfs:domain :Property ;
                rdfs:range xsd:dateTime ;
                skos:example "2014-04-30T10:39:53Z" ;
                rdfs:label "Date of creation" .


###  http://www.w3id.org/ppon/bppo#dateOfDeactivation
:dateOfDeactivation rdf:type owl:DatatypeProperty ;
                    rdfs:domain :Property ;
                    rdfs:range xsd:dateTime ;
                    rdfs:comment "Date as of which the property becomes obsolete. The property is maintained in the dictionary." ;
                    rdfs:label "Date of deactivation" .


###  http://www.w3id.org/ppon/bppo#dateOfLastChange
:dateOfLastChange rdf:type owl:DatatypeProperty ;
                  rdfs:domain :Property ;
                  rdfs:range xsd:dateTime ;
                  rdfs:comment "Date of validation of the last change request" ;
                  rdfs:label "Date of last change" .


###  http://www.w3id.org/ppon/bppo#dateOfRevision
:dateOfRevision rdf:type owl:DatatypeProperty ;
                rdfs:domain :Property ;
                rdfs:range xsd:dateTime ;
                rdfs:comment "Date of the revision" ;
                rdfs:label "Date of revision" .


###  http://www.w3id.org/ppon/bppo#dateOfVersion
:dateOfVersion rdf:type owl:DatatypeProperty ;
               rdfs:domain :Property ;
               rdfs:range xsd:dateTime ;
               rdfs:comment "Date of the version" ;
               rdfs:label "Date of version" .


###  http://www.w3id.org/ppon/bppo#definition
:definition rdf:type owl:DatatypeProperty ;
            rdfs:domain :Property ;
            rdfs:range xsd:language ;
            rdfs:comment "List of pairs (Definition of the property, language)" .


###  http://www.w3id.org/ppon/bppo#deprecationExplanation
:deprecationExplanation rdf:type owl:DatatypeProperty ;
                        rdfs:domain :Property ;
                        rdfs:range xsd:string ;
                        rdfs:comment "Sentence explaining the reason of the deprecation. Can explain how to convert values to conform to the new property. This explanation has to be written in international English (EN)" ;
                        rdfs:label "Deprecation explanation" .


###  http://www.w3id.org/ppon/bppo#description
:description rdf:type owl:DatatypeProperty ;
             rdfs:subPropertyOf owl:topDataProperty ;
             rdfs:domain :Property ;
             rdfs:range xsd:language ;
             rdfs:comment """List of pairs (Description of  the property, language)
This attribute is used to provide a plain language description of the property""" .


###  http://www.w3id.org/ppon/bppo#digitalFormat
:digitalFormat rdf:type owl:DatatypeProperty ;
               rdfs:domain :Property ;
               rdfs:comment "Pair for digital text type (precision, unit of measure). Precision is the number of significant digits" ;
               rdfs:label "Digital format" .


###  http://www.w3id.org/ppon/bppo#dimension
:dimension rdf:type owl:DatatypeProperty ;
           rdfs:domain :Property ;
           rdfs:range xsd:string ;
           rdfs:comment "In case of a physical quantity, dimension according to ISO 80000. This attribute allows the dimension to be machine readable. As all physical quantities are derived from 7 base quantities, it is provided with the power attached to a basic dimension in the following order and with one space between each." .


###  http://www.w3id.org/ppon/bppo#hasGUID
:hasGUID rdf:type owl:DatatypeProperty ;
         rdfs:domain :Property ;
         rdfs:range xsd:anyURI ;
         skos:example "936DA01F-9ABD-4D9D-80C7-02AF85C822A8" ;
         rdfs:comment             "globally unique identifier generated using an algorithm in conformity with standard ISO/IEC 11578:1996" ;
         rdfs:label "globally unique identifier" .


###  http://www.w3id.org/ppon/bppo#hasName
:hasName rdf:type owl:DatatypeProperty ;
         rdfs:domain :Property ;
         rdfs:range xsd:language ;
         rdfs:comment """List of pairs (Name of the property and language).
This attribute can be used to add synonyms for different domains""" .


###  http://www.w3id.org/ppon/bppo#isDynamicProperty
:isDynamicProperty rdf:type owl:DatatypeProperty ;
                   rdfs:subPropertyOf owl:topDataProperty ;
                   rdfs:domain :Property ;
                   rdfs:range xsd:boolean ;
                   rdfs:comment "If this is a dynamic property, the value will be expressed as a formula" ;
                   rdfs:label "Dynamic property" .


###  http://www.w3id.org/ppon/bppo#numberOfValues
:numberOfValues rdf:type owl:DatatypeProperty ;
                rdfs:subPropertyOf owl:topDataProperty ;
                rdfs:domain :Property ;
                rdfs:range xsd:integer ;
                rdfs:comment "This attribute provides information about the number of values to provide. It may be one value or a table of values (equivalent to ifcPropertyTableValue in EN ISO 16739). In case of a table value, the number of values represent the number of rows of a 2 columns table" ;
                rdfs:label "Number of values" .


###  http://www.w3id.org/ppon/bppo#physicalQuantity
:physicalQuantity rdf:type owl:DatatypeProperty ;
                  rdfs:domain :Property ;
                  rdfs:comment "List of Pairs (Physical quantity | Language). Physical quantities are expressed in International System (SI) units Non-physical quantities such as text are expressed with the value \"without\". This is equivalent to a measure in EN ISO 16739 and ISO 10303" ;
                  rdfs:label "Physical quantity" .


###  http://www.w3id.org/ppon/bppo#revisionNumber
:revisionNumber rdf:type owl:DatatypeProperty ;
                rdfs:domain :Property ;
                rdfs:range xsd:integer ;
                rdfs:comment "This revision number allows tracking of minor changes eg new translation, changes of typos. If the version number changes, the revision number starts again at 1" .


###  http://www.w3id.org/ppon/bppo#units
:units rdf:type owl:DatatypeProperty ;
       rdfs:domain :Property ;
       rdfs:range xsd:string ;
       rdfs:comment "a unit to represent a scale that enables a value to be measured. It can be possible to use this attribute to explain there is no unit attached to the property by using “unitless”" ;
       rdfs:label "Units" .


###  http://www.w3id.org/ppon/bppo#versionNumber
:versionNumber rdf:type owl:DatatypeProperty ;
               rdfs:domain :Property ;
               rdfs:range xsd:integer ;
               skos:example "2" ;
               rdfs:comment  "This version number allows tracking of major changes essentially a change of the domain" ;
               rdfs:label "Version number" .


#################################################################
#    Classes
#################################################################

###  http://purl.org/dc/elements/1.1/Language
dc:Language rdf:type owl:Class .


###  http://www.w3id.org/bpo#Attribute
bpo:Attribute rdf:type owl:Class .


###  http://www.w3id.org/bpo#Product
bpo:Product rdf:type owl:Class .


###  http://www.w3id.org/bpo#RangedAttribute
bpo:RangedAttribute rdf:type owl:Class .


###  http://www.w3id.org/ppon/bppo#InterconnectedDictionary
:InterconnectedDictionary rdf:type owl:Class ;
                          rdfs:comment "Interconnected Dictionary is a dictionary following this standard and connected using specific attributes and interconnected to other interconnected dictionaries." .


###  http://www.w3id.org/ppon/bppo#Property
:Property rdf:type owl:Class ;
          rdfs:subClassOf [ rdf:type owl:Restriction ;
                            owl:onProperty skos:related ;
                            owl:someValuesFrom bpo:Attribute
                          ] ,
                          [ rdf:type owl:Restriction ;
                            owl:onProperty skos:related ;
                            owl:someValuesFrom bpo:RangedAttribute
                          ] ;
          rdfs:comment "A class represents the properties of product used in the construction." ,
                       "a property is defined as inherent or acquired feature (ISO/DIS 6707-1)" .


###  http://www.w3id.org/ppon/bppo#PropertyGroup
:PropertyGroup rdf:type owl:Class ;
               rdfs:comment "A container enabling the properties to be prearranged or organized. A Property Set as defined is ISO 16739 is a group of properties, but a group of properties is not necessarily a Property Set." .


###  http://www.w3id.org/ppon/bppo#Status
:Status rdf:type owl:Class ;
        rdfs:comment "The status of the property during its life cycle." .


#################################################################
#    Individuals
#################################################################

###  http://www.w3id.org/ppon/bppo#Active
:Active rdf:type owl:NamedIndividual ,
                 :Status .


###  http://www.w3id.org/ppon/bppo#Inactive
:Inactive rdf:type owl:NamedIndividual ,
                   :Status .


###  Generated by the OWL API (version 4.5.9.2019-02-01T07:24:44Z) https://github.com/owlcs/owlapi
